verified-ocaml/automatic/Bytecode/MetaSpecProof.v
@@ -11,9 +11,11 @@ From OCamlInterp.Manual.Bytecode.Interpret Require Import MetaSpec.
 Lemma handler_unique_mod_errors :
   forall (i : instruction)
          (h1 h2 : Z -> state -> step_result),
-    handler_correct h1 (clight_of i) (pre_of i)
+    handler_correct h1 (clight_of i)
+      (fun e m s ard => instr_wfb i = true /\ pre_of i e m s ard)
       (P_error_of i) (P_halt_of i) (P_ccall_of i) ->
-    handler_correct h2 (clight_of i) (pre_of i)
+    handler_correct h2 (clight_of i)
+      (fun e m s ard => instr_wfb i = true /\ pre_of i e m s ard)
       (P_error_of i) (P_halt_of i) (P_ccall_of i) ->
     forall s, em_eq (h1 s.(pc) s) (h2 s.(pc) s).
 Proof.
